\documentclass[border=0.2cm]{standalone}

\usepackage[english]{babel}
\usepackage{csquotes}
\usepackage{calc}
\usepackage[absolute,overlay]{textpos}
\usepackage{graphicx}
\usepackage{subcaption}
\usepackage{wrapfig}
\usepackage{subfig}
\usepackage{mathtools}
\usepackage{amsmath,amscd}
\usepackage{amsfonts}
\usepackage{amsthm}
\usepackage{comment}
\usepackage{siunitx}
\usepackage{MnSymbol,wasysym}
\usepackage{array}
\usepackage{qrcode}
\usepackage{physics}
\usepackage{tikz}
\usepackage{tikz-3dplot}
\usepackage[outline]{contour} % glow around text
\usepackage{xcolor}
\usepackage[<options>]{animate}
\pagestyle{empty}
\begin{document}

\color{black}
$\begin{array}{l|l|l|l}
\text{Process}                      &
\text{Kalman filter (KF)}           & 
\text{Extended Kalman filter (EKF)} & 
\text{Unscented Kalman filter (UKF)} \\

\hline 
& & & \\

\text{Prediction} &
\mathbf{\bar x} = \mathbf{Fx} + \mathbf{Bu} & 
\mathbf{\bar x} = f(\mathbf x, \mathbf u),\, \mathbf F = {\frac{\partial{f(\mathbf x_t, \mathbf u_t)}}{\partial{\mathbf x}}}\biggr|_{{\mathbf x_t},{\mathbf u_t}} & 
\mathbf{\bar x} = \sum w^m\boldsymbol{\mathcal Y},\, \boldsymbol{\mathcal Y} = f(\boldsymbol\chi) \\

\text{(Time update)} &
\mathbf{\bar P} = \mathbf{FPF}^\mathsf{T}+\mathbf Q  & 
\mathbf{\bar P} = \mathbf{FPF}^\mathsf{T}+\mathbf Q  &
\mathbf{\bar P} = \sum w^c(\boldsymbol{\mathcal Y} - \mathbf{\bar x})(\boldsymbol{\mathcal Y} - \mathbf{\bar x})^\mathsf T+\mathbf Q \\

\hline
& & & \\

& & & \boldsymbol\mu_z = \sum w^m\boldsymbol{\mathcal{Z}}, \boldsymbol{\mathcal Z} =  h(\boldsymbol{\mathcal{Y}}) \\

\text{Update} &
\textbf{y} = \mathbf z - \mathbf{H \bar{x}} & 
\textbf{y} = \mathbf z - h(\bar{\mathbf x}),\, \mathbf H = \frac{\partial{h(\bar{\mathbf x}_t)}}{\partial{\bar{\mathbf x}}}\biggr|_{\bar{\mathbf x}_t} &
\mathbf y = \mathbf z - \boldsymbol\mu_z \\

\text{(Measurement update)} &
\mathbf S = \mathbf{H\bar PH}^\mathsf{T} + \mathbf R & 
\mathbf S = \mathbf{H\bar PH}^\mathsf{T} + \mathbf R & 
\mathbf P_z = \sum w^c{(\boldsymbol{\mathcal Z}-\boldsymbol\mu_z)(\boldsymbol{\mathcal{Z}}-\boldsymbol\mu_z)^\mathsf{T}} + \mathbf R \\

& 
\mathbf K = \mathbf{\bar PH}^\mathsf T \mathbf S^{-1} & 
\mathbf K = \mathbf{\bar PH}^\mathsf T \mathbf S^{-1} &
\mathbf K = \left[\sum w^c(\boldsymbol{\mathcal Y}-\bar{\mathbf x})(\boldsymbol{\mathcal{Z}}-\boldsymbol\mu_z)^\mathsf{T}\right] \mathbf P_z^{-1} \\

&
\mathbf x = \mathbf{\bar x} + \mathbf{Ky} & 
\mathbf x = \mathbf{\bar x} + \mathbf{Ky} &
\mathbf x = \mathbf{\bar x} + \mathbf{Ky} \\

&
\mathbf P = (\mathbf{I}-\mathbf{KH})\mathbf{\bar{P}} & 
\mathbf P = (\mathbf{I}-\mathbf{KH})\mathbf{\bar{P}} &
\mathbf P = \bar{\mathbf P} - \mathbf{KP_z}\mathbf{K}^\mathsf{T}
\end{array}$

\end{document}